examples/pkc_checker/array/scpog_arrayProgScript.sml
@@ -1,0 +1,1116 @@
+(*
+  This refines scpog_list to use arrays
+*)
+open preamble basis UnsafeProofTheory cnf_scpogTheory scpog_listTheory scpog_parsingTheory blastLib;
+
+val _ = new_theory "scpog_arrayProg"
+
+val _ = diminish_srw_ss ["ABBREV"]
+
+(* TODO: move *)
+Theorem ALL_DISTINCT_MAP_FST_toSortedAList:
+  ALL_DISTINCT (MAP FST (toSortedAList t))
+Proof
+  `SORTED $< (MAP FST (toSortedAList t))` by
+    simp[SORTED_toSortedAList]>>
+  pop_assum mp_tac>>
+  match_mp_tac SORTED_ALL_DISTINCT>>
+  simp[irreflexive_def]
+QED
+
+Theorem MAP_FST_enumerate:
+  MAP FST (enumerate k ls) = GENLIST ($+ k) (LENGTH ls)
+Proof
+  rw[LIST_EQ_REWRITE,LENGTH_enumerate]>>
+  simp[EL_MAP,LENGTH_enumerate,EL_enumerate]
+QED
+
+Theorem ALL_DISTINCT_MAP_FST_enumerate:
+  ALL_DISTINCT (MAP FST (enumerate k ls))
+Proof
+  simp[MAP_FST_enumerate,ALL_DISTINCT_GENLIST]
+QED
+
+(* replace in miscTheory *)
+Theorem MEM_enumerate_IMP:
+  ∀ls k.
+  MEM (i,e) (enumerate k ls) ⇒ MEM e ls
+Proof
+  Induct_on`ls`>>fs[miscTheory.enumerate_def]>>rw[]>>
+  metis_tac[]
+QED
+
+Theorem ALOOKUP_enumerate:
+  ∀ls k x.
+  ALOOKUP (enumerate k ls) x =
+  if k ≤ x ∧ x < LENGTH ls + k then SOME (EL (x-k) ls) else NONE
+Proof
+  Induct>>rw[miscTheory.enumerate_def]>>
+  `x-k = SUC(x-(k+1))` by DECIDE_TAC>>
+  simp[]
+QED
+
+val _ = translation_extends"UnsafeProg";
+
+(* Pure translation of SCPOG checker *)
+val _ = register_type``:scpstep``;
+val _ = register_type``:'a spt``;
+
+val _ = translate insert_def;
+
+(* TODO: make sure these get inlined! *)
+val _ = translate w8z_def;
+val _ = translate w8o_def;
+val _ = translate index_def;
+
+val w8z_v_thm = fetch "-" "w8z_v_thm";
+val w8o_v_thm = fetch "-" "w8o_v_thm";
+
+val index_side_def = fetch "-" "index_side_def"
+
+val index_side = Q.prove(`
+  !x. index_side x ⇔ T`,
+  simp[index_side_def]>>
+  intLib.ARITH_TAC) |> update_precondition;
+
+val _ = process_topdecs `
+  exception Fail string;
+` |> append_prog
+
+fun get_exn_conv name =
+  EVAL ``lookup_cons (Short ^name) ^(get_env (get_ml_prog_state ()))``
+  |> concl |> rand |> rand |> rand
+
+val fail = get_exn_conv ``"Fail"``
+
+Definition Fail_exn_def:
+  Fail_exn v = (∃s sv. v = Conv (SOME ^fail) [sv] ∧ STRING_TYPE s sv)
+End
+
+Definition eq_w8o_def:
+  eq_w8o v ⇔ v = w8o
+End
+
+val _ = translate (eq_w8o_def |> SIMP_RULE std_ss [w8o_def]);
+
+val every_one_arr = process_topdecs`
+  fun every_one_arr carr cs =
+  case cs of [] => True
+  | c::cs =>
+    if eq_w8o (Unsafe.w8sub carr (index c)) then every_one_arr carr cs
+    else False` |> append_prog
+
+Definition format_failure_def:
+  format_failure (lno:num) s =
+  strlit "c Checking failed at line: " ^ toString lno ^ strlit ". Reason: " ^ s ^ strlit"\n"
+End
+
+val _ = translate format_failure_def;
+
+Definition unwrap_TYPE_def:
+  unwrap_TYPE P x y =
+  ∃z. x = SOME z ∧ P z y
+End
+
+val delete_literals_sing_arr_def = process_topdecs`
+  fun delete_literals_sing_arr lno i carr cs =
+  case cs of
+    [] => 0
+  | c::cs =>
+    if eq_w8o (Unsafe.w8sub carr (index c)) then
+      delete_literals_sing_arr lno i carr cs
+    else
+      if every_one_arr carr cs then ~c
+      else raise Fail (format_failure lno ("clause at index not empty or singleton after reduction: "  ^ Int.toString i))` |> append_prog
+
+val xlet_autop = xlet_auto >- (TRY( xcon) >> xsimpl)
+
+Theorem update_resize_LUPDATE[simp]:
+  LENGTH Clist > index h ⇒
+  update_resize Clist w8z v (index h) = LUPDATE v (index h) Clist
+Proof
+  rw[update_resize_def]
+QED
+
+Theorem every_one_arr_spec:
+  ∀ls lsv.
+  (LIST_TYPE INT) ls lsv ∧
+  EVERY ($> (LENGTH Clist) o index) ls
+  ⇒
+  app (p : 'ffi ffi_proj)
+    ^(fetch_v "every_one_arr" (get_ml_prog_state()))
+    [Carrv; lsv]
+    (W8ARRAY Carrv Clist)
+    (POSTv v.
+      W8ARRAY Carrv Clist *
+      &BOOL (EVERY (λi. any_el (index i) Clist w8z = w8o) ls) v)
+Proof
+  Induct>>rw[]>>
+  xcf "every_one_arr" (get_ml_prog_state ())>>
+  fs[LIST_TYPE_def]
+  >-
+    (xmatch>>xcon>>xsimpl)>>
+  xmatch>>
+  rpt xlet_autop>>
+  fs[eq_w8o_def,any_el_ALT]>>
+  xif
+  >-
+    (xapp>>xsimpl)>>
+  xcon>> xsimpl
+QED
+
+val raise_tac =
+  rpt xlet_autop>>
+  xraise>>xsimpl>>
+  simp[unwrap_TYPE_def,Fail_exn_def]>>
+  metis_tac[];
+
+Theorem delete_literals_sing_arr_spec:
+  ∀ls lsv lno lnov i iv.
+  NUM lno lnov ∧
+  NUM i iv ∧
+  (LIST_TYPE INT) ls lsv ∧
+  EVERY ($> (LENGTH Clist) o index) ls
+  ⇒
+  app (p : 'ffi ffi_proj)
+    ^(fetch_v "delete_literals_sing_arr" (get_ml_prog_state()))
+    [lnov; iv; Carrv; lsv]
+    (W8ARRAY Carrv Clist)
+    (POSTve
+      (λv. W8ARRAY Carrv Clist *
+        &unwrap_TYPE INT (delete_literals_sing_list Clist ls) v)
+      (λe. &(Fail_exn e ∧ delete_literals_sing_list Clist ls = NONE)))
+Proof
+  Induct>>simp[delete_literals_sing_list_def]>>
+  rpt strip_tac>>
+  xcf "delete_literals_sing_arr" (get_ml_prog_state ())
+  >- (
+    fs[LIST_TYPE_def]>>
+    xmatch>>
+    xlit
+    >- (
+      simp[unwrap_TYPE_def]>>
+      xsimpl)>>
+    xsimpl)>>
+  fs[LIST_TYPE_def]>> xmatch>>
+  rpt xlet_autop >>
+  fs[eq_w8o_def,any_el_ALT]>>
+  xif
+  >- (
+    xapp>>xsimpl>>
+    metis_tac[])>>
+  xlet_auto>>
+  gvs[any_el_ALT]>>
+  xif
+  >- (
+    xapp>>xsimpl>>simp[unwrap_TYPE_def]>>
+    metis_tac[])>>
+  IF_CASES_TAC>- metis_tac[NOT_EVERY]>>
+  raise_tac
+QED
+
+val is_rup_arr_aux = process_topdecs`
+  fun is_rup_arr_aux lno pred fml ls c carr =
+    case ls of
+      [] =>
+        raise Fail (format_failure lno
+          ("failed to derive clause by RUP"))
+    | (i::is) =>
+    if Array.length fml <= i then
+      raise Fail (format_failure lno
+        ("no clause at index: " ^ Int.toString i))
+    else
+    case Unsafe.sub fml i of
+      None => raise Fail (format_failure lno
+        ("no clause at index (maybe deleted): " ^ Int.toString i))
+    | Some ct =>
+      if pred ct then
+        let val nl = delete_literals_sing_arr lno i carr (fst ct) in
+        if nl = 0 then c
+        else
+          (Unsafe.w8update carr (index nl) w8o;
+          is_rup_arr_aux lno pred fml is (nl::c) carr)
+        end
+      else
+        raise Fail (format_failure lno
+          ("wrong clause type at index: " ^ Int.toString i))
+         ` |> append_prog
+
+(* For every literal in every clause and their negations,
+  the index is bounded above by n *)
+Definition bounded_fml_def:
+  bounded_fml n fmlls ⇔
+  EVERY (λCopt.
+    case Copt of
+      NONE => T
+    | SOME (C,t) => EVERY ($> n o index) C ∧ EVERY ($> n o index o $~) C
+    ) fmlls
+End
+
+Theorem delete_literals_sing_list_MEM:
+  ∀C.
+  delete_literals_sing_list ls C = SOME x ∧ x ≠ 0
+  ⇒
+  MEM (-x) C
+Proof
+  Induct>>rw[delete_literals_sing_list_def] >> simp[] >>
+  CCONTR_TAC >> fs [] >> rw []
+QED
+
+Overload "ctag_TYPE" = ``PAIR_TYPE (LIST_TYPE INT) NUM``
+Overload "pred_TYPE" = ``ctag_TYPE --> BOOL``;
+
+Theorem is_rup_arr_aux_spec:
+  ∀ls lsv c cv fmlv fmlls fml Carrv Clist lno lnov.
+  NUM lno lnov ∧
+  (LIST_TYPE NUM) ls lsv ∧
+  (LIST_TYPE INT) c cv ∧
+  LIST_REL (OPTION_TYPE ctag_TYPE) fmlls fmllsv ∧
+  pred_TYPE pred predv ∧
+  bounded_fml (LENGTH Clist) fmlls
+  ⇒
+  app (p : 'ffi ffi_proj)
+    ^(fetch_v "is_rup_arr_aux" (get_ml_prog_state()))
+    [lnov; predv; fmlv; lsv; cv; Carrv]
+    (ARRAY fmlv fmllsv * W8ARRAY Carrv Clist)
+    (POSTve
+      (λv. ARRAY fmlv fmllsv *
+        (SEP_EXISTS Clist'.
+          W8ARRAY Carrv Clist' *
+          &unwrap_TYPE ($= o SND)
+          (is_rup_list_aux pred fmlls ls c Clist) Clist'
+        ) *
+        &unwrap_TYPE
+          (LIST_TYPE INT o FST)
+          (is_rup_list_aux pred fmlls ls c Clist) v)
+      (λe. ARRAY fmlv fmllsv *
+        &(Fail_exn e ∧ is_rup_list_aux pred fmlls ls c Clist = NONE)))
+Proof
+  Induct>>
+  rw[]>>
+  xcf "is_rup_arr_aux" (get_ml_prog_state ())>>
+  simp[is_rup_list_aux_def]
+  >- (
+    fs[LIST_TYPE_def]>> xmatch>>
+    raise_tac)>>
+  fs[LIST_TYPE_def]>>
+  xmatch>>
+  rpt xlet_autop>>
+  xif
+  >- (
+    `any_el h fmlls NONE = NONE` by (
+      simp[any_el_ALT]>>
+      drule LIST_REL_LENGTH>>
+      gvs[])>>
+    raise_tac>>
+    simp[unwrap_TYPE_def]>>
+    metis_tac[])>>
+  xlet_autop>>
+  `OPTION_TYPE ctag_TYPE (EL h fmlls) (EL h fmllsv)` by fs[LIST_REL_EL_EQN]>>
+  TOP_CASE_TAC
+  >- (
+    fs[any_el_ALT]>>
+    reverse (Cases_on`EL h fmlls`)>-
+      (fs[IS_SOME_DEF]>>
+      drule LIST_REL_LENGTH>>
+      gvs[])>>
+    fs[OPTION_TYPE_def]>>
+    xmatch>>
+    raise_tac)>>
+  fs[any_el_ALT,OPTION_TYPE_def]>>
+  xmatch>>
+  xlet_autop>>
+  reverse xif
+  >- raise_tac>>
+  rpt xlet_autop>>
+  xlet_auto
+  >- (
+    xsimpl>>
+    fs[bounded_fml_def,EVERY_EL]>>
+    first_x_assum(qspec_then`h` mp_tac)>>simp[]>>
+    TOP_CASE_TAC>>rw[])
+  >- (
+    xsimpl>>rw[]>> simp[]>>
+    metis_tac[])>>
+  fs[unwrap_TYPE_def]>>
+  xlet_autop>>
+  xif
+  >- (
+    xcon>>xsimpl>>
+    simp[SUM_TYPE_def])>>
+  rpt xlet_autop>>
+  `index z < LENGTH Clist ∧ WORD8 w8o w8o_v` by (
+    fs[w8o_v_thm]>>
+    fs[bounded_fml_def,EVERY_EL]>>
+    first_x_assum(qspec_then`h` assume_tac)>>rfs[AllCasePreds()]>>
+    drule delete_literals_sing_list_MEM>>fs[]>>
+    simp[MEM_EL]>>
+    rw[]>>
+    pop_assum mp_tac>>
+    rpt (first_x_assum drule)>>
+    rw[]>>
+    pop_assum sym_sub_tac>>fs[])>>
+  rpt xlet_autop>>
+  xapp>>
+  xsimpl>>
+  qexists_tac`fmlls`>>qexists_tac`z::c`>>
+  simp[LIST_TYPE_def]>>
+  metis_tac[]
+QED
+
+val set_array = process_topdecs`
+  fun set_array carr v cs =
+  case cs of [] => ()
+  | (c::cs) =>
+    (Unsafe.w8update carr (index c) v;
+    set_array carr v cs)` |> append_prog
+
+Theorem set_array_spec:
+  ∀c cv Carrv Clist.
+  (LIST_TYPE INT) c cv ∧
+  WORD8 v vv ∧
+  EVERY ($> (LENGTH Clist) o index) c
+  ⇒
+  app (p : 'ffi ffi_proj)
+    ^(fetch_v "set_array" (get_ml_prog_state()))
+    [Carrv; vv; cv]
+    (W8ARRAY Carrv Clist)
+    (POSTv uv.
+          W8ARRAY Carrv (set_list Clist v c))
+Proof
+  Induct>>
+  rw[]>>
+  xcf "set_array" (get_ml_prog_state ())>>
+  rw[set_list_def]>>
+  fs[LIST_TYPE_def]
+  >- (xmatch>>xcon>>xsimpl)>>
+  xmatch>>
+  rpt xlet_autop>>
+  xapp>>
+  xsimpl
+QED
+
+val is_rup_arr = process_topdecs`
+  fun is_rup_arr lno pred fml ls c carr =
+    (set_array carr w8o c;
+    set_array carr w8z (is_rup_arr_aux lno pred fml ls c carr);
+    carr)`
+    |> append_prog
+
+Theorem LENGTH_set_list_bound[simp]:
+  ∀c Clist.
+  EVERY ($> (LENGTH Clist) ∘ index) c ⇒
+  LENGTH (set_list Clist v c) = LENGTH Clist
+Proof
+  Induct>>simp[set_list_def]
+QED
+
+(* a version of this is true even if x, h are not bounded *)
+Theorem update_resize_twice:
+  index x < LENGTH Clist ∧ index h < LENGTH Clist ⇒
+  update_resize (update_resize Clist w8z w8o (index x)) w8z w8o (index h) =
+  update_resize (update_resize Clist w8z w8o (index h)) w8z w8o (index x)
+Proof
+  rw[update_resize_def]>>
+  Cases_on`x=h`>>simp[]>>
+  `index x ≠ index h` by metis_tac[index_11]>>
+  metis_tac[LUPDATE_commutes]
+QED
+
+Theorem set_list_update_resize:
+  ∀c Clist.
+  index x < LENGTH Clist ∧ EVERY ($> (LENGTH Clist) ∘ index) c ⇒
+  set_list Clist w8o (x::c) =
+  update_resize (set_list Clist w8o c) w8z w8o (index x)
+Proof
+  Induct>>rw[]>>fs[set_list_def]>>
+  Cases_on`x=h`>>simp[]
+  >-
+    (first_x_assum (qspec_then` LUPDATE w8o (index h) Clist` mp_tac)>>
+    simp[])
+  >>
+  dep_rewrite.DEP_ONCE_REWRITE_TAC[LUPDATE_commutes]>>
+  simp[index_11]
+QED
+
+Theorem is_rup_list_aux_length_bound:
+  ∀ls c Clist.
+  bounded_fml (LENGTH Clist) fmlls ∧
+  EVERY ($> (LENGTH Clist) ∘ index) c ∧
+  is_rup_list_aux pred fmlls ls c (set_list Clist w8o c) = SOME(d,r) ⇒
+    Abbrev (r = set_list Clist w8o d ∧
+    LENGTH r = LENGTH Clist ∧
+    EVERY ($> (LENGTH Clist) ∘ index) d)
+Proof
+  Induct>>rw[is_rup_list_aux_def,set_list_def]>>simp[]>>
+  gvs[AllCaseEqs()]
+  >-
+    simp[markerTheory.Abbrev_def]>>
+  first_x_assum irule>>
+  drule delete_literals_sing_list_MEM>> simp[]>>
+  strip_tac>>
+  fs[bounded_fml_def,EVERY_MEM,any_el_ALT]>>
+  first_x_assum(qspec_then`EL h fmlls` mp_tac)>>
+  impl_tac>- (
+    `h < LENGTH fmlls` by fs[]>>
+    metis_tac[MEM_EL])>>
+  simp[]>>strip_tac>>
+  qexists_tac`nl::c`>>
+  gvs[AllCasePreds()]>>
+  CONJ_TAC >- (
+    dep_rewrite.DEP_ONCE_REWRITE_TAC[set_list_update_resize]>>
+    simp[EVERY_MEM]>>
+    gvs[AllCasePreds()]>>
+    pop_assum drule>>
+    simp[]) >>
+  simp[]>>
+  rw[]
+  >- (
+    pop_assum drule>>
+    simp[])>>
+  metis_tac[]
+QED
+
+Theorem is_rup_arr_spec:
+  ∀ls lsv c cv fmlv fmlls Carrv Clist lno lnov.
+  NUM lno lnov ∧
+  (LIST_TYPE NUM) ls lsv ∧
+  (LIST_TYPE INT) c cv ∧
+  LIST_REL (OPTION_TYPE ctag_TYPE) fmlls fmllsv ∧
+  pred_TYPE pred predv ∧
+  bounded_fml (LENGTH Clist) fmlls ∧
+  EVERY ($> (LENGTH Clist) ∘ index) c
+  ⇒
+  app (p : 'ffi ffi_proj)
+    ^(fetch_v "is_rup_arr" (get_ml_prog_state()))
+    [lnov; predv; fmlv; lsv; cv; Carrv]
+    (ARRAY fmlv fmllsv * W8ARRAY Carrv Clist)
+    (POSTve
+      (λv. ARRAY fmlv fmllsv *
+          (SEP_EXISTS Clist'.
+          W8ARRAY Carrv Clist' *
+          &(unwrap_TYPE $=
+            (is_rup_list pred fmlls ls c Clist) Clist' ∧
+            LENGTH Clist = LENGTH Clist')
+          ) *
+        &unwrap_TYPE
+          (λv w. T)
+          (is_rup_list pred fmlls ls c Clist) v)
+      (λe. ARRAY fmlv fmllsv *
+        &(Fail_exn e ∧ is_rup_list pred fmlls ls c Clist = NONE)))
+Proof
+  rw[]>>
+  xcf "is_rup_arr" (get_ml_prog_state ())>>
+  `WORD8 w8z w8z_v ∧ WORD8 w8o w8o_v` by
+    simp[w8z_v_thm,w8o_v_thm]>>
+  xlet_autop>>
+  xlet_auto
+  >- (
+    xsimpl>>fs[])
+  >- (
+    simp[is_rup_list_def]>>
+    xsimpl>>
+    rw[]>>simp[]>>
+    metis_tac[])>>
+  fs[unwrap_TYPE_def]>>
+  simp[is_rup_list_def]>>
+  rw[]>>fs[]>>rw[]>>
+  TOP_CASE_TAC>>fs[]>>
+  drule is_rup_list_aux_length_bound>>
+  rpt (disch_then drule)>>
+  simp[markerTheory.Abbrev_def]>>
+  strip_tac>>
+  xlet_autop>>
+  xvar>>xsimpl
+QED
+
+val _ = translate list_max_def;
+val _ = translate list_max_index_def;
+
+(* bump up the length to a large number *)
+val resize_carr = process_topdecs`
+  fun resize_carr c carr =
+  let val lm = list_max_index c in
+    if Word8Array.length carr <= lm
+    then Word8Array.array (2*lm) w8z
+    else carr
+  end` |> append_prog
+
+Theorem resize_carr_spec:
+  (LIST_TYPE INT) c cv ⇒
+  app (p : 'ffi ffi_proj)
+    ^(fetch_v "resize_carr" (get_ml_prog_state()))
+    [cv; Carrv]
+    (W8ARRAY Carrv Clist)
+    (POSTv carrv.
+      W8ARRAY carrv (resize_Clist c Clist))
+Proof
+  rw[]>>
+  xcf "resize_carr" (get_ml_prog_state ())>>
+  rpt xlet_autop>>
+  simp[resize_Clist_def]>>xif
+  >- (
+    xlet_autop>>xapp>>
+    xsimpl>>
+    metis_tac[w8z_v_thm])>>
+  xvar>>
+  xsimpl
+QED
+
+val insert_one_arr = process_topdecs`
+  fun insert_one_arr lno tag fml i c =
+  case Array.lookup fml None i of
+    None =>
+      Array.updateResize fml None i (Some (c,tag))
+  | Some cc =>
+    raise Fail (format_failure lno "cannot overwrite existing clause at id: "^ Int.toString i)` |> append_prog;
+
+(* TODO: copied *)
+Theorem LIST_REL_update_resize:
+  LIST_REL R a b ∧ R a1 b1 ∧ R a2 b2 ⇒
+  LIST_REL R (update_resize a a1 a2 n) (update_resize b b1 b2 n)
+Proof
+  rw[update_resize_def]
+  >- (
+    match_mp_tac EVERY2_LUPDATE_same>>
+    fs[])
+  >- fs[LIST_REL_EL_EQN]
+  >- fs[LIST_REL_EL_EQN]>>
+  match_mp_tac EVERY2_LUPDATE_same>>
+  simp[]>>
+  match_mp_tac EVERY2_APPEND_suff>>
+  fs[LIST_REL_EL_EQN]>>rw[]>>
+  fs[EL_REPLICATE]
+QED
+
+Theorem insert_one_arr_spec:
+  NUM lno lnov ∧
+  LIST_REL (OPTION_TYPE ctag_TYPE) fmlls fmllsv ∧
+  NUM tag tagv ∧
+  (LIST_TYPE INT) c cv ∧
+  NUM i iv
+  ⇒
+  app (p : 'ffi ffi_proj)
+    ^(fetch_v "insert_one_arr" (get_ml_prog_state()))
+    [lnov; tagv; fmlv; iv; cv]
+    (ARRAY fmlv fmllsv)
+    (POSTve
+      (λv.
+        SEP_EXISTS fmllsv'.
+        ARRAY v fmllsv' *
+        &(case insert_one_list tag fmlls i c of NONE => F
+        | SOME fmlls' =>
+          LIST_REL (OPTION_TYPE ctag_TYPE) fmlls' fmllsv'))
+      (λe.
+        ARRAY fmlv fmllsv *
+        & (Fail_exn e ∧
+          insert_one_list tag fmlls i c  = NONE)))
+Proof
+  rw[insert_one_list_def]>>
+  xcf"insert_one_arr"(get_ml_prog_state ())>>
+  xlet_autop>>
+  xlet_auto>>
+  `OPTION_TYPE ctag_TYPE (any_el i fmlls NONE) v'` by (
+    rw[any_el_ALT]>>
+    fs[LIST_REL_EL_EQN,OPTION_TYPE_def])>>
+  reverse (Cases_on`any_el i fmlls NONE`)>>gvs[OPTION_TYPE_def]>>
+  xmatch
+  >- raise_tac>>
+  rpt xlet_autop>>
+  xapp>>xsimpl>>
+  irule_at Any LIST_REL_update_resize>>
+  gvs[OPTION_TYPE_def,PAIR_TYPE_def]
+QED
+
+val insert_list_arr = process_topdecs`
+  fun insert_list_arr lno tag fml i ls =
+  case ls of [] => fml
+  | c::cs =>
+    insert_list_arr lno tag (insert_one_arr lno tag fml i c) (i+1) cs` |> append_prog;
+
+Theorem ARRAY_refl:
+  (ARRAY fml fmllsv ==>> ARRAY fml fmllsv) ∧
+  (ARRAY fml fmllsv ==>> ARRAY fml fmllsv * GC)
+Proof
+  xsimpl
+QED
+
+Theorem insert_list_arr_spec:
+  ∀ls lsv i iv fmlls fmllsv fmlv.
+  NUM lno lnov ∧
+  LIST_REL (OPTION_TYPE ctag_TYPE) fmlls fmllsv ∧
+  NUM tag tagv ∧
+  LIST_TYPE (LIST_TYPE INT) ls lsv ∧
+  NUM i iv
+  ⇒
+  app (p : 'ffi ffi_proj)
+    ^(fetch_v "insert_list_arr" (get_ml_prog_state()))
+    [lnov; tagv; fmlv; iv; lsv]
+    (ARRAY fmlv fmllsv)
+    (POSTve
+      (λv.
+        SEP_EXISTS fmllsv'.
+        ARRAY v fmllsv' *
+        &(case insert_list_list tag fmlls i ls of NONE => F
+        | SOME fmlls' =>
+          LIST_REL (OPTION_TYPE ctag_TYPE) fmlls' fmllsv'))
+      (λe.
+        SEP_EXISTS fmlv fmllsv.
+        ARRAY fmlv fmllsv *
+        & (Fail_exn e ∧
+          insert_list_list tag fmlls i ls = NONE)))
+Proof
+  Induct>>
+  rw[insert_list_list_def]>>
+  xcf"insert_list_arr"(get_ml_prog_state ())>>
+  gvs[LIST_TYPE_def]>>
+  xmatch
+  >- (xvar>>xsimpl)>>
+  rpt xlet_autop
+  >-(
+    xsimpl>>
+    rw[]>>
+    metis_tac[ARRAY_refl])>>
+  gvs[AllCasePreds()]>>
+  xapp>>xsimpl
+QED
+
+val _ = register_type``:scpog_conf``;
+val _ = register_type``:prob_conf``;
+
+val res = translate var_lit_def;
+val res = translate lookup_def;
+val res = translate is_data_var_def;
+val res = translate is_data_ext_lit_run_def;
+val res = translate declare_root_def;
+
+val res = translate is_structural_def;
+val res = translate is_forward_def;
+val res = translate is_strfwd_def;
+
+Definition every_not_is_fresh_def:
+  every_not_is_fresh pc sc c =
+    EVERY (λi. ¬is_fresh pc sc (var_lit i)) c
+End
+
+val res = translate is_fresh_def;
+val res = translate every_not_is_fresh_def;
+
+val delete_arr = process_topdecs`
+  fun delete_arr i fml =
+    if Array.length fml <= i then ()
+    else
+      (Unsafe.update fml i None)` |> append_prog
+
+Theorem LUPDATE_outside:
+  ∀ls n.
+  LENGTH ls ≤ n ⇒
+  LUPDATE x n ls = ls
+Proof
+  Induct>>rw[LUPDATE_DEF]
+QED
+
+Theorem delete_arr_spec:
+  NUM i iv
+  ⇒
+  app (p : 'ffi ffi_proj)
+    ^(fetch_v "delete_arr" (get_ml_prog_state()))
+    [iv; fmlv]
+    (ARRAY fmlv fmllsv)
+    (POSTv resv.
+      &UNIT_TYPE () resv *
+      ARRAY fmlv (LUPDATE (Conv (SOME (TypeStamp "None" 2)) []) i fmllsv))
+Proof
+  rw[]>>
+  xcf "delete_arr" (get_ml_prog_state ())>>
+  rpt xlet_autop>>
+  xif>- (
+    xcon>>xsimpl>>
+    DEP_REWRITE_TAC[LUPDATE_outside]>>
+    simp[])>>
+  xlet_auto >- (xcon>>xsimpl)>>
+  xapp>>xsimpl>>
+  first_x_assum (irule_at Any)>>
+  simp[]
+QED
+
+val res = translate is_adel_def;
+
+Definition is_adel_sc_def:
+  is_adel_sc sc = is_adel sc.root
+End
+
+val res = translate is_adel_sc_def;
+
+val arb_delete_arr = process_topdecs`
+  fun arb_delete_arr lno sc ls fml =
+    case ls of [] => ()
+  | (i::is) =>
+    case Array.lookup fml None i of
+    None =>
+      raise Fail (format_failure lno "missing id for arbitrary deletion: "^ Int.toString i)
+  | Some ctag =>
+    if is_adel_sc sc ctag
+    then
+      (delete_arr i fml; arb_delete_arr lno sc is fml)
+    else
+    raise Fail (format_failure lno "invalid arbitrary deletion at id: "^ Int.toString i)` |> append_prog;
+
+Theorem arb_delete_arr_spec:
+  ∀ls lsv fmlls fmlv fmllsv.
+  NUM lno lnov ∧
+  CNF_SCPOG_SCPOG_CONF_TYPE sc scv ∧
+  LIST_TYPE NUM ls lsv ∧
+  LIST_REL (OPTION_TYPE ctag_TYPE) fmlls fmllsv
+  ⇒
+  app (p : 'ffi ffi_proj)
+    ^(fetch_v "arb_delete_arr" (get_ml_prog_state()))
+    [lnov; scv; lsv; fmlv]
+    (ARRAY fmlv fmllsv)
+    (POSTve
+      (λv.
+        SEP_EXISTS fmllsv'.
+        ARRAY fmlv fmllsv' *
+        &(UNIT_TYPE () v ∧
+        case arb_delete_list sc ls fmlls of NONE => F
+        | SOME fmlls' =>
+          LIST_REL (OPTION_TYPE ctag_TYPE) fmlls' fmllsv'))
+      (λe.
+        SEP_EXISTS fmllsv'.
+        ARRAY fmlv fmllsv' *
+        & (Fail_exn e ∧
+          arb_delete_list sc ls fmlls = NONE)))
+Proof
+  Induct>>rw[arb_delete_list_def]>>
+  xcf "arb_delete_arr" (get_ml_prog_state ())>>
+  gvs[LIST_TYPE_def]>>xmatch
+  >- (xcon>>xsimpl)>>
+  rpt xlet_autop>>
+  xlet_auto>>
+  `OPTION_TYPE ctag_TYPE (any_el h fmlls NONE) v'` by (
+    rw[any_el_ALT]>>
+    fs[LIST_REL_EL_EQN,OPTION_TYPE_def])>>
+  gvs[OPTION_TYPE_SPLIT]>>xmatch
+  >- raise_tac>>
+  rpt xlet_autop>>
+  gvs[is_adel_sc_def]>>
+  reverse xif
+  >- raise_tac>>
+  xlet_autop>>
+  xapp>>xsimpl>>
+  match_mp_tac EVERY2_LUPDATE_same>>
+  simp[OPTION_TYPE_def]
+QED
+
+Definition mk_backward_def:
+  mk_backward sc = is_backward sc.root
+End
+
+val res = translate is_root_def;
+val res = translate is_backward_def;
+val res = translate mk_backward_def;
+val res = translate strfwd_tag_def;
+
+Definition is_input_tag_def:
+  is_input_tag tag = (tag = input_tag)
+End
+
+val res = translate is_input_tag_def;
+
+val res = translate check_pro_def;
+val res = translate FOLDL;
+val res = translate mk_BN_def;
+val res = translate mk_BS_def;
+val res = translate inter_def;
+val res = translate union_def;
+val res = translate big_disjoint_union_def;
+val res = translate get_node_vars_def;
+val res = translate mk_Ev_disj_def;
+val res = translate mk_sko_def;
+val res = translate mk_pro_def;
+val res = translate declare_pro_def;
+
+val res = translate check_sum_def;
+val res = translate mk_sum_def;
+val res = translate big_union_def;
+val res = translate mk_Ev_def;
+val res = translate declare_sum_def;
+
+val res = translate is_proj_lit_run_def;
+val res = translate check_sko_def;
+val res = translate declare_sko_def;
+
+Definition mk_cl_def:
+  mk_cl l1 (l2:int) = [-l1;-l2]
+End
+val res = translate mk_cl_def;
+
+val check_scpstep_arr = process_topdecs`
+  fun check_scpstep_arr lno scpstep pc fml sc carr =
+  case scpstep of
+    Skip => (fml,sc,carr)
+  | Root l =>
+      (case declare_root pc sc l of
+        None => raise Fail (format_failure lno "invalid root declaration")
+      | Some sc' => (fml,sc',carr))
+  | Rupadd b n c i0 =>
+    (let val carr = resize_carr c carr
+        val u = is_rup_arr lno (is_strfwd b) fml i0 c carr in
+      if every_not_is_fresh pc sc c
+      then
+        (insert_one_arr lno (strfwd_tag b) fml n c, sc, carr)
+      else raise Fail (format_failure lno "clause has fresh variable")
+    end)
+  | Rupdel n i0 =>
+    (case Array.lookup fml None n of
+      None => raise Fail (format_failure lno "invalid RUP deletion")
+    | Some (c,tag) =>
+      if is_input_tag tag then
+        let
+          val u1 = delete_arr n fml
+          val u2 = is_rup_arr lno (mk_backward sc) fml i0 c carr in
+          (fml, sc, carr)
+        end
+      else raise Fail (format_failure lno "invalid deletion tag for clause"))
+  | Arbdel ls =>
+    (arb_delete_arr lno sc ls fml; (fml,sc,carr))
+  | Declpro n v ls =>
+    (case declare_pro pc sc v ls of
+      Some (cs,sc') =>
+        (insert_list_arr lno 1 fml n cs, sc', carr)
+    | _ =>
+      raise Fail (format_failure lno "Product node freshness/variable checks failed"))
+  | Declsum n v l1 l2 i0 =>
+    (let
+      val c = mk_cl l1 l2
+      val carr = resize_carr c carr
+      val u = is_rup_arr lno is_structural fml i0 c carr in
+      (case declare_sum pc sc v l1 l2 of
+        Some (cs,sc') =>
+          (insert_list_arr lno 1 fml n cs,sc',carr)
+      | _ =>
+        raise Fail (format_failure lno "Sum node freshness/variable checks failed"))
+    end)
+  | Declsko n v ls =>
+    (case declare_sko pc sc v ls of
+      Some (cT,csF,sc') =>
+        (insert_list_arr lno 5 (insert_one_arr lno 0 fml n cT) (n+1) csF, sc',carr)
+    | _ =>
+      raise Fail (format_failure lno "Skolem node freshness/variable checks failed"))`
+  |> append_prog;
+
+val CNF_SCPOG_SCPSTEP_TYPE_def = fetch "-" "CNF_SCPOG_SCPSTEP_TYPE_def";
+
+Theorem OPTION_TYPE_SPLIT:
+  OPTION_TYPE a x v ⇔
+  (x = NONE ∧ v = Conv (SOME (TypeStamp "None" 2)) []) ∨
+  (∃y vv. x = SOME y ∧ v = Conv (SOME (TypeStamp "Some" 2)) [vv] ∧ a y vv)
+Proof
+  Cases_on`x`>>rw[OPTION_TYPE_def]
+QED
+
+Theorem PAIR_TYPE_SPLIT:
+  PAIR_TYPE a b x v ⇔
+  ∃x1 x2 v1 v2. x = (x1,x2) ∧ v = Conv NONE [v1; v2] ∧ a x1 v1 ∧ b x2 v2
+Proof
+  Cases_on`x`>>EVAL_TAC>>rw[]
+QED
+
+Theorem check_scpstep_arr_spec:
+  NUM lno lnov ∧
+  CNF_SCPOG_SCPSTEP_TYPE scpstep scpstepv ∧
+  CNF_SCPOG_PROB_CONF_TYPE pc pcv ∧
+  CNF_SCPOG_SCPOG_CONF_TYPE sc scv ∧
+  LIST_REL (OPTION_TYPE ctag_TYPE) fmlls fmllsv ∧
+  bounded_fml (LENGTH Clist) fmlls
+  ⇒
+  app (p : 'ffi ffi_proj)
+    ^(fetch_v "check_scpstep_arr" (get_ml_prog_state()))
+    [lnov; scpstepv; pcv; fmlv; scv; Carrv]
+    (ARRAY fmlv fmllsv * W8ARRAY Carrv Clist)
+    (POSTve
+      (λv.
+        SEP_EXISTS v1 v2 v3.
+          &(v = Conv NONE [v1; v2; v3]) *
+          (* v1 points to the array
+             v2 is SCP config
+             v3 points to the byte array
+          *)
+          (SEP_EXISTS fmllsv' clist'.
+            ARRAY v1 fmllsv' *
+            W8ARRAY v3 clist' *
+            &(
+            case check_scpstep_list scpstep pc fmlls sc Clist of
+              NONE => F
+            | SOME (fmlls', sc' , Clist') =>
+                bounded_fml (LENGTH Clist') fmlls' ∧
+                LIST_REL (OPTION_TYPE ctag_TYPE) fmlls' fmllsv' ∧
+                Clist' = clist' ∧
+                LENGTH Clist ≤ LENGTH Clist'
+            ))
+      )
+      (λe.
+        SEP_EXISTS fmllsv'.
+        ARRAY fmlv fmllsv' *
+        &(Fail_exn e ∧
+        check_scpstep_list scpstep pc fmlls sc Clist = NONE)))
+Proof
+  rw[check_scpstep_list_def]>>
+  xcf "check_scpstep_arr" (get_ml_prog_state ())>>
+  Cases_on`scpstep`>>fs[CNF_SCPOG_SCPSTEP_TYPE_def]
+  >- ( (* Skip *)
+    xmatch >>
+    xcon>>xsimpl)
+  >- ( (* Root *)
+    xmatch>>
+    xlet_autop>>
+    gvs[OPTION_TYPE_SPLIT]
+    >- (
+      xmatch>>
+      raise_tac)>>
+    xmatch>>
+    xcon>>xsimpl)
+  >- ( (* RupAdd *)
+    xmatch>>
+    xlet_autop>>
+    xlet`(POSTv f.
+      W8ARRAY carrv (resize_Clist l Clist) * ARRAY fmlv fmllsv * &(pred_TYPE (is_strfwd b) f))`
+    >- (
+      assume_tac (fetch "-" "is_strfwd_v_thm" |> Q.GEN`a` |> Q.ISPEC `LIST_TYPE INT`)>>
+      drule Arrow_IMP_app_basic>>
+      disch_then drule>>
+      simp[GSYM app_def]>>
+      simp[cf_app_def,local_def,PULL_EXISTS]>>rw[]>>
+      first_x_assum (irule_at (Pos (el 4)))>>
+      xsimpl>>
+      CONJ_TAC >-
+        metis_tac[ml_monad_translatorBaseTheory.EMP_STAR_GC,ml_monad_translatorBaseTheory.H_STAR_GC_SAT_IMP]>>
+      EVAL_TAC)>>
+    xlet_auto
+    >- (
+      xsimpl>>
+      cheat)
+    >- xsimpl>>
+    xlet_autop>>
+    fs[unwrap_TYPE_def,every_not_is_fresh_def]>>
+    reverse xif
+    >- (
+      `¬EVERY (λi. ¬is_fresh pc sc (var_lit i)) l` by metis_tac[NOT_EVERY,o_DEF]>>
+      raise_tac)>>
+    xlet_autop>>
+    xlet`POSTve
+      (λv.
+           SEP_EXISTS fmllsv'.
+             ARRAY v fmllsv' * W8ARRAY carrv Clist' *
+             &case insert_one_list (strfwd_tag b) fmlls n l of
+               NONE => F
+             | SOME fmlls' => LIST_REL (OPTION_TYPE ctag_TYPE) fmlls' fmllsv')
+      (λe.
+           ARRAY fmlv fmllsv *
+           &(Fail_exn e ∧ insert_one_list (strfwd_tag b) fmlls n l = NONE))`
+    >- (
+      xapp>>xsimpl>>
+      rpt (first_x_assum (irule_at Any))>>
+      simp[])
+    >- xsimpl>>
+    gvs[AllCasePreds()]>>
+    xcon>>xsimpl>>
+    cheat)
+  >- ( (* RupDel *)
+    xmatch>>
+    rpt xlet_autop>>
+    `OPTION_TYPE ctag_TYPE (any_el n fmlls NONE) v'` by (
+      rw[any_el_ALT]>>
+      fs[LIST_REL_EL_EQN,OPTION_TYPE_def])>>
+    gvs[OPTION_TYPE_SPLIT,PAIR_TYPE_SPLIT]>>xmatch
+    >- raise_tac>>
+    xlet_autop>>
+    gvs[is_input_tag_def]>>
+    reverse xif
+    >- raise_tac>>
+    rpt xlet_autop>>
+    qmatch_goalsub_abbrev_tac`ARRAY fmlv fmllsv'`>>
+    xlet`(POSTv f.
+      (ARRAY fmlv fmllsv' * W8ARRAY Carrv Clist) * &(pred_TYPE (is_backward sc.root) f))`
+    >- (
+      assume_tac (fetch "-" "mk_backward_v_thm")>>
+      drule Arrow_IMP_app_basic>>
+      disch_then drule>>
+      simp[GSYM app_def]>>
+      simp[cf_app_def,local_def,PULL_EXISTS,mk_backward_def]>>rw[]>>
+      first_x_assum (irule_at (Pos (el 4)))>>
+      xsimpl>>
+      CONJ_TAC >-
+        metis_tac[ml_monad_translatorBaseTheory.EMP_STAR_GC,ml_monad_translatorBaseTheory.H_STAR_GC_SAT_IMP]>>
+      EVAL_TAC)>>
+    qmatch_goalsub_abbrev_tac`is_rup_list pred _ ls c Clist`>>
+    `bounded_fml (LENGTH Clist) (LUPDATE NONE n fmlls)` by cheat>>
+    `LIST_REL (OPTION_TYPE ctag_TYPE) (LUPDATE NONE n fmlls) fmllsv'` by cheat>>
+    xlet`POSTve
+            (λv.
+                 ARRAY fmlv fmllsv' *
+                 (SEP_EXISTS Clist'.
+                    W8ARRAY Carrv Clist' *
+                    &(unwrap_TYPE $= (is_rup_list pred (LUPDATE NONE n fmlls) ls c Clist)
+                       Clist' ∧ LENGTH Clist = LENGTH Clist')) *
+                 &unwrap_TYPE (λv w. T) (is_rup_list pred (LUPDATE NONE n fmlls) ls c Clist) v)
+            (λe.
+                 ARRAY fmlv fmllsv' *
+                 &(Fail_exn e ∧ is_rup_list pred (LUPDATE NONE n fmlls) ls c Clist = NONE))`
+    >- (
+      xapp>>xsimpl>>
+      cheat)
+    >- xsimpl>>
+    gvs[unwrap_TYPE_def]>>
+    xcon>>xsimpl)
+  >- (  (* ArbDel *)
+    xmatch>>
+    xlet`
+      POSTve
+        (λv.
+             SEP_EXISTS fmllsv'.
+               ARRAY fmlv fmllsv' * W8ARRAY Carrv Clist *
+               &(UNIT_TYPE () v ∧
+                case arb_delete_list sc l fmlls of
+                  NONE => F
+                | SOME fmlls' => LIST_REL (OPTION_TYPE ctag_TYPE) fmlls' fmllsv'))
+        (λe.
+             SEP_EXISTS fmllsv'.
+               ARRAY fmlv fmllsv' *
+               &(Fail_exn e ∧ arb_delete_list sc l fmlls = NONE))`
+    >- (
+      xapp>>xsimpl>>
+      rpt (first_x_assum (irule_at Any))>>
+      simp[])
+    >- xsimpl>>
+    gvs[AllCasePreds()]>>xcon>>xsimpl>>
+    cheat)
+  >- ( (* DeclPro *)
+    xmatch>>
+    rpt xlet_autop>>
+    gvs[OPTION_TYPE_SPLIT,PAIR_TYPE_SPLIT]>>
+    xmatch
+    >- raise_tac>>
+    xlet`POSTve
+      (λv.
+           SEP_EXISTS fmllsv'.
+             ARRAY v fmllsv' * W8ARRAY Carrv Clist *
+             &case insert_list_list 1 fmlls n x1 of
+               NONE => F
+             | SOME fmlls' => LIST_REL (OPTION_TYPE ctag_TYPE) fmlls' fmllsv')
+      (λe.
+           SEP_EXISTS fmlv' fmllsv'.
+             ARRAY fmlv' fmllsv' *
+             &(Fail_exn e ∧ insert_list_list 1 fmlls n x1 = NONE))`
+    >- (
+      xapp>>xsimpl>>
+      rpt(first_x_assum (irule_at Any))>>
+      simp[]>>
+      rw[]>>
+      qexists_tac`x`>>qexists_tac`x'`>>xsimpl)
+    >-
+      cheat)>>
+  cheat
+QED
+
+val _ = export_theory();
